lint: verify that all expected theorems are present
We add a check to the linting script called check-theorems that ensures that all HOL-Light
proofs provide the expected set of theorems depending on the
architecture.

Signed-off-by: Andreas Hatziiliou <andreas.hatziiliou@savoirfairelinux.com>

proofs/hol_light/x86_64/proofs/ntttobytes_avx2_asm.ml
@@ -277,16 +277,16 @@ let LENGTH_MLKEM_TOBYTES_TMC =
   REWRITE_CONV[mlkem_tobytes_tmc] `LENGTH mlkem_tobytes_tmc`
   |> CONV_RULE(RAND_CONV LENGTH_CONV);;
 
-let MLKEM_TOBYTES_POSTAMBLE_LENGTH = new_definition
-  `MLKEM_TOBYTES_POSTAMBLE_LENGTH = 1`;;
+let MLKEM_NTTTOBYTES_POSTAMBLE_LENGTH = new_definition
+  `MLKEM_NTTTOBYTES_POSTAMBLE_LENGTH = 1`;;
 
-let MLKEM_TOBYTES_CORE_END = new_definition
-  `MLKEM_TOBYTES_CORE_END = LENGTH mlkem_tobytes_tmc - MLKEM_TOBYTES_POSTAMBLE_LENGTH`;;
+let MLKEM_NTTTOBYTES_CORE_END = new_definition
+  `MLKEM_NTTTOBYTES_CORE_END = LENGTH mlkem_tobytes_tmc - MLKEM_NTTTOBYTES_POSTAMBLE_LENGTH`;;
 
 let LENGTH_SIMPLIFY_CONV =
   REWRITE_CONV[LENGTH_MLKEM_TOBYTES_TMC;
-              MLKEM_TOBYTES_CORE_END;
-              MLKEM_TOBYTES_POSTAMBLE_LENGTH] THENC
+              MLKEM_NTTTOBYTES_CORE_END;
+              MLKEM_NTTTOBYTES_POSTAMBLE_LENGTH] THENC
   NUM_REDUCE_CONV THENC REWRITE_CONV [ADD_0];;
 
 let avx_order = new_definition
@@ -301,7 +301,7 @@ let permute_list = new_definition
 let BIT_BOUND = BITBLAST_RULE
   `!x:int16. val x < 3329 ==> ~bit 12 x /\ ~bit 13 x /\ ~bit 14 x /\ ~bit 15 x`;;
 
-let MLKEM_TOBYTES_CORRECT = prove(
+let MLKEM_NTTTOBYTES_CORRECT = prove(
   `!r a (l:int16 list) pc.
         aligned 32 a /\
         aligned 32 r /\
@@ -313,7 +313,7 @@ let MLKEM_TOBYTES_CORRECT = prove(
                   read RIP s = word pc /\
                   C_ARGUMENTS [r; a] s /\
                   read (memory :> bytes(a, 512)) s = num_of_wordlist l)
-             (\s. read RIP s = word (pc + MLKEM_TOBYTES_CORE_END) /\
+             (\s. read RIP s = word (pc + MLKEM_NTTTOBYTES_CORE_END) /\
                   (LENGTH l = 256
                    ==> (!i. i < LENGTH l ==> val(EL i l) < 3329)
                    ==> read(memory :> bytes(r, 384)) s =
@@ -396,7 +396,7 @@ let MLKEM_TOBYTES_CORRECT = prove(
   ABBREV_TAC `twae = &2:real` THEN REAL_ARITH_TAC
 );;
 
-let MLKEM_TOBYTES_NOIBT_SUBROUTINE_CORRECT = prove
+let MLKEM_NTTTOBYTES_NOIBT_SUBROUTINE_CORRECT = prove
 (`!r a (l:int16 list) pc.
         aligned 32 a /\
         aligned 32 r /\
@@ -421,12 +421,12 @@ let MLKEM_TOBYTES_NOIBT_SUBROUTINE_CORRECT = prove
                MAYCHANGE [memory :> bytes(r, 384)])`,
   CONV_TAC LENGTH_SIMPLIFY_CONV THEN
   X86_PROMOTE_RETURN_NOSTACK_TAC mlkem_tobytes_tmc
-    (CONV_RULE LENGTH_SIMPLIFY_CONV MLKEM_TOBYTES_CORRECT));;
+    (CONV_RULE LENGTH_SIMPLIFY_CONV MLKEM_NTTTOBYTES_CORRECT));;
 
 (* NOTE: This must be kept in sync with the CBMC specification
  * in mlkem/src/native/x86_64/src/arith_native_x86_64.h *)
 
-let MLKEM_TOBYTES_SUBROUTINE_CORRECT = prove
+let MLKEM_NTTTOBYTES_SUBROUTINE_CORRECT = prove
 (`!r a (l:int16 list) pc.
         aligned 32 a /\
         aligned 32 r /\
@@ -449,7 +449,7 @@ let MLKEM_TOBYTES_SUBROUTINE_CORRECT = prove
                        num_of_wordlist (MAP word_zx (permute_list l):(12 word)list)))
              (MAYCHANGE [RSP] ,, MAYCHANGE_REGS_AND_FLAGS_PERMITTED_BY_ABI ,,
                MAYCHANGE [memory :> bytes(r, 384)])`,
-  MATCH_ACCEPT_TAC(ADD_IBT_RULE MLKEM_TOBYTES_NOIBT_SUBROUTINE_CORRECT));;
+  MATCH_ACCEPT_TAC(ADD_IBT_RULE MLKEM_NTTTOBYTES_NOIBT_SUBROUTINE_CORRECT));;
 
 (* ------------------------------------------------------------------------- *)
 (* Constant-time and memory safety proof.                                    *)
@@ -461,10 +461,10 @@ needs "mlkem_native/x86_64/proofs/subroutine_signatures.ml";;
 let full_spec,public_vars = mk_safety_spec
     ~keep_maychanges:true
     (assoc "mlkem_tobytes" subroutine_signatures)
-    MLKEM_TOBYTES_CORRECT
+    MLKEM_NTTTOBYTES_CORRECT
     mlkem_tobytes_TMC_EXEC;;
 
-let MLKEM_TOBYTES_SAFE = time prove
+let MLKEM_NTTTOBYTES_SAFE = time prove
  (`exists f_events.
        forall e r a pc.
            aligned 32 a /\
@@ -479,7 +479,7 @@ let MLKEM_TOBYTES_SAFE = time prove
                     C_ARGUMENTS [r; a] s /\
                     read events s = e)
                (\s.
-                    read RIP s = word (pc + MLKEM_TOBYTES_CORE_END) /\
+                    read RIP s = word (pc + MLKEM_NTTTOBYTES_CORE_END) /\
                     (exists e2.
                          read events s = APPEND e2 e /\
                          e2 = f_events a r pc /\
@@ -495,7 +495,7 @@ let MLKEM_TOBYTES_SAFE = time prove
   CONV_TAC LENGTH_SIMPLIFY_CONV THEN
   PROVE_SAFETY_SPEC_TAC ~public_vars:public_vars mlkem_tobytes_TMC_EXEC);;
 
-let MLKEM_TOBYTES_NOIBT_SUBROUTINE_SAFE = time prove
+let MLKEM_NTTTOBYTES_NOIBT_SUBROUTINE_SAFE = time prove
  (`exists f_events.
        forall e r a pc stackpointer returnaddress.
           aligned 32 a /\
@@ -523,10 +523,10 @@ let MLKEM_TOBYTES_NOIBT_SUBROUTINE_SAFE = time prove
                            [r,384; stackpointer,8]))
                (\s s'. true)`,
   X86_PROMOTE_RETURN_NOSTACK_TAC mlkem_tobytes_tmc
-    (CONV_RULE LENGTH_SIMPLIFY_CONV MLKEM_TOBYTES_SAFE) THEN
+    (CONV_RULE LENGTH_SIMPLIFY_CONV MLKEM_NTTTOBYTES_SAFE) THEN
   DISCHARGE_SAFETY_PROPERTY_TAC);;
 
-let MLKEM_TOBYTES_SUBROUTINE_SAFE = time prove
+let MLKEM_NTTTOBYTES_SUBROUTINE_SAFE = time prove
  (`exists f_events.
        forall e r a pc stackpointer returnaddress.
           aligned 32 a /\
@@ -553,4 +553,4 @@ let MLKEM_TOBYTES_SUBROUTINE_SAFE = time prove
                            [a,512; r,384; stackpointer,8]
                            [r,384; stackpointer,8]))
                (\s s'. true)`,
-  MATCH_ACCEPT_TAC(ADD_IBT_RULE MLKEM_TOBYTES_NOIBT_SUBROUTINE_SAFE));;
+  MATCH_ACCEPT_TAC(ADD_IBT_RULE MLKEM_NTTTOBYTES_NOIBT_SUBROUTINE_SAFE));;
